theories/completeness.v
@@ -1,0 +1,55 @@
+Require Export domain_semantics.
+
+Definition val_ok ρ0 ρ1 Γ :=
+  forall i A, lookup i Γ A -> SEq A (ρ0 i) (ρ1 i).
+
+Definition SemWt Γ a A := forall ρ0 ρ1, val_ok ρ0 ρ1 Γ -> exists d0 d1,
+      compile ρ0 a d0 /\ compile ρ1 a d1 /\ SEq A d0 d1.
+
+Lemma val_ok_ext ρ0 ρ1 Γ d0 d1 A :
+  SEq A d0 d1 ->
+  val_ok ρ0 ρ1 Γ ->
+  val_ok (d0.:ρ0) (d1.:ρ1) (A :: Γ).
+Proof.
+  move => h0 h1 n B.
+  inversion 1; subst.
+  - done.
+  - sfirstorder.
+Qed.
+
+
+Notation "Γ ⊨ a ∈ A" := (SemWt Γ a A) (at level 70).
+
+Lemma ST_Var Γ i A :
+  lookup i Γ A ->
+  Γ ⊨ VarTm i ∈ A.
+Proof.
+  hauto ctrs:compile unfold:val_ok.
+Qed.
+
+Lemma ST_Fun Γ b A B :
+  A :: Γ ⊨ b ∈ B ->
+  Γ ⊨ Abs b ∈ Fun A B.
+Proof.
+  move => h ρ0 ρ1 hρ.
+  do 2 eexists.
+  repeat split.
+  constructor. constructor.
+  simpl. move => d d' hd.
+  move : val_ok_ext hρ hd; repeat move/[apply].
+  move => {}/h.
+  hauto q:on ctrs:ap.
+Qed.
+
+Lemma ST_App Γ b a A B :
+  Γ ⊨ b ∈ Fun A B ->
+  Γ ⊨ a ∈ A ->
+  Γ ⊨ App b a ∈ B.
+Proof.
+  move => h0 h1 ρ0 ρ1 hρ.
+  move : h0 (hρ) => /[apply].
+  move => [b0][b1][hb0][hb1]hbe.
+  move : h1 (hρ) => /[apply].
+  move => [a0][a1][ha0][ha1]hae.
+  hauto lq:on unfold:FunSpace ctrs:compile.
+Qed.
